Rule jumpi_neq with constraints

optimizations/jumpi_neq.v
@@ -1,5 +1,6 @@
 Require Import bbv.Word.
 Require Import Nat. 
+Require Import Bool.
 Require Import Coq.NArith.NArith.
 
 Require Import Coq.Logic.FunctionalExtensionality.
@@ -61,11 +62,17 @@ Import Context.
 Require Import FORVES2.tools_types.
 Import ToolsTypes.
 
+Require Import FORVES2.context.
+Import Context.
+
+Require Import FORVES2.context_facts.
+Import ContextFacts.
+
 Require Import List.
 Import ListNotations.
 
 
-Module Opt_jumpi_eval.
+Module Opt_jumpi_neq.
 
 
 Definition val_diff_zero (arg: sstack_val) (fcmp: sstack_val_cmp_t) 
@@ -78,8 +85,10 @@ match follow_in_smap arg maxid sb with
   end.
 
 
-(* JUMPI(Dest,B) = Dest if B is constant and B <> 0 *)
-Definition optimize_jumpi_eval_sbinding : opt_smap_value_type := 
+(* JUMPI(Dest,B) = Dest if B <> 0 
+ B <> 0 if it is a different constant or if it's implied by the constraints
+*)
+Definition optimize_jumpi_neq_sbinding : opt_smap_value_type := 
 fun (val: smap_value) =>
 fun (tools: Tools_1.tools_1_t) =>
 fun (sb: sbindings) =>
@@ -89,7 +98,9 @@ fun (ops: stack_op_instr_map) =>
   let fcmp := Tools_1.sstack_val_cmp tools in
   match val with
   | SymOp JUMPI [arg1; arg2] => 
-      if val_diff_zero arg2 fcmp maxid sb ctx ops then
+      if (val_diff_zero arg2 fcmp maxid sb ctx ops || 
+          chk_neq_wrt_ctx ctx arg2 (Val WZero))
+      then
         (SymBasicVal arg1, true)
       else
         (val, false)
@@ -97,17 +108,17 @@ fun (ops: stack_op_instr_map) =>
   end.
 
 
-Lemma optimize_jumpi_eval_sbinding_smapv_valid:
-opt_smapv_valid_snd optimize_jumpi_eval_sbinding.
+Lemma optimize_jumpi_neq_sbinding_smapv_valid:
+opt_smapv_valid_snd optimize_jumpi_neq_sbinding.
 Proof.
 unfold opt_smapv_valid_snd.
 intros ctx n tools sb val val' flag.
 intros Hvalid_smapv_val Hvalid_sb Hoptm_sbinding.
-unfold optimize_jumpi_eval_sbinding in Hoptm_sbinding.
+unfold optimize_jumpi_neq_sbinding in Hoptm_sbinding.
 destruct (val) as [basicv|pushtagv|label args|offset smem|key sstrg|
   offset size smem] eqn: eq_val; 
    try inject_rw Hoptm_sbinding eq_val'.
-destruct label eqn: eq_label; try inject_rw Hoptm_sbinding eq_val'. try 
+destruct label eqn: eq_label; try inject_rw Hoptm_sbinding eq_val'. 
 (* JUMPI *)
 destruct args as [|arg1 r1] eqn: eq_args; try inject_rw Hoptm_sbinding eq_val'.
 destruct r1 as [|arg2 r2] eqn: eq_r1; try inject_rw Hoptm_sbinding eq_val'.
@@ -118,16 +129,19 @@ unfold Tools_1.sstack_val_cmp in Hoptm_sbinding.
 remember sstack_val_cmp as fcmp.
 assert(Hsafe_sstack_val_cmp:=H_sstack_val_cmp_snd).
 
-destruct (val_diff_zero arg2 fcmp n sb ctx evm_stack_opm)
-  eqn: eq_val_diff_zero_arg1.
-* injection Hoptm_sbinding as eq_val' eq_flag.
+destruct (val_diff_zero arg2 fcmp n sb ctx evm_stack_opm
+          || chk_neq_wrt_ctx ctx arg2 (Val WZero)) 
+  eqn: arg1_diff_zero.
+* (* B <> 0 *) 
+  injection Hoptm_sbinding as eq_val' eq_flag.
   rewrite <- eq_val'.
   simpl in Hvalid_smapv_val. unfold valid_stack_op_instr in Hvalid_smapv_val.
   simpl in Hvalid_smapv_val.
   destruct Hvalid_smapv_val as [_ [Hvalid_arg1 [Hvalid_arg2 _]]].
   simpl.
   assumption.
-* injection Hoptm_sbinding as eq_val' eq_flag.
+* (* B == 0 *) 
+  injection Hoptm_sbinding as eq_val' eq_flag.
   rewrite <- eq_val'.
   assumption.
 Qed.
@@ -144,21 +158,21 @@ reflexivity.
 Qed.
 
 
-Lemma optimize_jumpi_eval_sbinding_snd:
-opt_sbinding_snd optimize_jumpi_eval_sbinding.
+Lemma optimize_jumpi_neq_sbinding_snd:
+opt_sbinding_snd optimize_jumpi_neq_sbinding.
 Proof.
 unfold opt_sbinding_snd.
 intros val val' tools sb maxidx ctx idx flag 
   Hvalid Hoptm_sbinding.
 split.
 - (* valid_sbindings *)
-  apply valid_bindings_snd_opt with (val:=val)(opt:=optimize_jumpi_eval_sbinding)
+  apply valid_bindings_snd_opt with (val:=val)(opt:=optimize_jumpi_neq_sbinding)
     (tools:=tools)(flag:=flag)(ctx:=ctx); try assumption.
-  apply optimize_jumpi_eval_sbinding_smapv_valid. 
+  apply optimize_jumpi_neq_sbinding_smapv_valid. 
     
 - (* evaluation is preserved *) 
   intros model mem strg exts v His_model Heval_orig.
-  unfold optimize_jumpi_eval_sbinding in Hoptm_sbinding.
+  unfold optimize_jumpi_neq_sbinding in Hoptm_sbinding.
   pose proof (Hvalid_maxidx  maxidx idx val sb evm_stack_opm
       Hvalid) as eq_maxidx_idx.
   destruct val as [vv|vv|label args|offset smem|key sstrg|offset seze smem]
@@ -177,8 +191,9 @@ split.
   remember sstack_val_cmp as fcmp.
   assert(Hsafe_sstack_val_cmp:=H_sstack_val_cmp_snd).
 
-  destruct (val_diff_zero arg2 fcmp idx sb ctx evm_stack_opm) 
-    eqn: eq_val_diff_z_arg2.
+  destruct (val_diff_zero arg2 fcmp idx sb ctx evm_stack_opm
+            || chk_neq_wrt_ctx ctx arg2 (Val WZero))
+    eqn: eq_arg2_neq_zero.
   + (* arg2  <> WZero *)
     injection Hoptm_sbinding as eq_val' _. 
     rewrite <- eq_val'.
@@ -198,34 +213,61 @@ split.
     simpl in Hvalid_smap_value.
     destruct (Hvalid_smap_value) as [_ [Hvalid_arg1 [Hvalid_arg2 _ ]]].
     fold valid_bindings in Hvalid_bindings_sb.
+ 
 
-    unfold val_diff_zero in eq_val_diff_z_arg2. 
-    destruct (follow_in_smap arg2 idx sb) as [fsmv|] eqn: eq_follow_arg2; try discriminate.
-    destruct fsmv as [svm] eqn: eq_fsmv.
-    destruct svm as [val2|pushtagv|label args'|offset smem|key' sstrg|
-    offset size smem] eqn: eq_svm; try discriminate.
-    destruct val2 as [v2|_a|_b] eqn: eq_val2; try discriminate.
-    rewrite -> Bool.negb_true_iff in  eq_val_diff_z_arg2.
+    apply orb_prop in eq_arg2_neq_zero.
+    destruct eq_arg2_neq_zero as [eq_arg2_neq_zero|eq_arg2_neq_zero].
+    * (* arg2 is constant <> 0 *)
+      unfold val_diff_zero in eq_arg2_neq_zero. 
+      destruct (follow_in_smap arg2 idx sb) as [fsmv|] eqn: eq_follow_arg2; try discriminate.
+      destruct fsmv as [svm] eqn: eq_fsmv.
+      destruct svm as [val2|pushtagv|label args'|offset smem|key' sstrg|
+        offset size smem] eqn: eq_svm; try discriminate.
+      destruct val2 as [v2|_a|_b] eqn: eq_val2; try discriminate.
+      rewrite -> Bool.negb_true_iff in  eq_arg2_neq_zero.
 
-    rewrite -> eq_maxid in eval_arg2.
-    simpl in eval_arg2.
-    rewrite -> eq_follow_arg2 in eval_arg2.
-    injection eval_arg2 as eq_varg2_v2.
-    rewrite <- eq_varg2_v2 in Heval_orig.
-    pose proof (evm_jumpi_not_zero exts varg1 v2 eq_val_diff_z_arg2) as Hjumpi.
-    simpl in Hjumpi. injection Heval_orig as Heval_orig.
-    rewrite -> Hjumpi in Heval_orig.
-    rewrite <- Heval_orig.
+      rewrite -> eq_maxid in eval_arg2.
+      simpl in eval_arg2.
+      rewrite -> eq_follow_arg2 in eval_arg2.
+      injection eval_arg2 as eq_varg2_v2.
+      rewrite <- eq_varg2_v2 in Heval_orig.
+      pose proof (evm_jumpi_not_zero exts varg1 v2 eq_arg2_neq_zero) as Hjumpi.
+      simpl in Hjumpi. injection Heval_orig as Heval_orig.
+      rewrite -> Hjumpi in Heval_orig.
+      rewrite <- Heval_orig.
     
-    unfold eval_sstack_val.
-    rewrite <- eval_sstack_val'_freshvar.
-    apply eval_sstack_val'_preserved_when_depth_extended.
-    rewrite -> eval'_maxidx_indep_eq with (m:=idx).
-    assumption.
+      unfold eval_sstack_val.
+      rewrite <- eval_sstack_val'_freshvar.
+      apply eval_sstack_val'_preserved_when_depth_extended.
+      rewrite -> eval'_maxidx_indep_eq with (m:=idx).
+      assumption.
+    * (* arg2 <> 0 by constraints *) 
+      apply chk_neq_wrt_ctx_snd with (model:=model)(mem:=mem)(strg:=strg)
+        (exts:=exts)(maxidx:=maxidx)(sb:=sb)(ops:=evm_stack_opm) 
+        in eq_arg2_neq_zero; try assumption.
+      destruct eq_arg2_neq_zero as [v1 [v2 [Heval_arg2 [Heval_zero Hneq_v1_v2]]]].
+      rewrite -> eval_sstack_val_const in Heval_zero.
+      injection Heval_zero as eq_v2.
+      rewrite <- eq_v2 in Hneq_v1_v2.
+      unfold eval_sstack_val in Heval_arg2.
+      apply eval_sstack_val'_preserved_when_depth_extended in eval_arg2.
+      rewrite -> eval'_maxidx_indep_eq with (m:=maxidx) in eval_arg2.
+      rewrite -> eval_arg2 in Heval_arg2.
+      injection Heval_arg2 as eq_v1_varg2.
+      rewrite <- eq_v1_varg2 in Hneq_v1_v2.
+      injection Heval_orig as Heval_orig.
+      rewrite -> Hneq_v1_v2 in Heval_orig.
+      rewrite <- Heval_orig.
+
+      unfold eval_sstack_val.
+      rewrite <- eval_sstack_val'_freshvar.
+      apply eval_sstack_val'_preserved_when_depth_extended.
+      rewrite -> eval'_maxidx_indep_eq with (m:=idx).
+      assumption.    
   + (* arg2 = WZero *)
     injection Hoptm_sbinding as eq_val' _.
     rewrite <- eq_val'.
     assumption.
 Qed.
 
-End Opt_jumpi_eval.
+End Opt_jumpi_neq.
