block_equiv_checker.v
@@ -148,8 +148,8 @@ Require Import FORVES2.optimizations.mem_solver.
 Import Opt_mem_solver.
 Require Import FORVES2.optimizations.strg_solver.
 Import Opt_strg_solver.
-Require Import FORVES2.optimizations.jumpi_eval.
-Import Opt_jumpi_eval.
+Require Import FORVES2.optimizations.jumpi_neq.
+Import Opt_jumpi_neq.
 
 Require Import FORVES2.symbolic_execution.
 Import SymbolicExecution.
@@ -237,6 +237,7 @@ Require Import FORVES2.tools_types.
 Import ToolsTypes.
 
 From Coq Require Import Lists.List. Import ListNotations.
+
 
 Module BlockEquivChecker.
 
@@ -434,7 +435,7 @@ Inductive available_optimization_step :=
 
 | OPT_mem_solver
 | OPT_strg_solver
-| OPT_jumpi_eval
+| OPT_jumpi_neq
 .
 
 
@@ -509,7 +510,7 @@ match tag with
 
 | OPT_mem_solver => OpEntry optimize_mem_solver_sbinding optimize_mem_solver_sbinding_snd
 | OPT_strg_solver => OpEntry optimize_strg_solver_sbinding optimize_strg_solver_sbinding_snd
-| OPT_jumpi_eval => OpEntry optimize_jumpi_eval_sbinding optimize_jumpi_eval_sbinding_snd
+| OPT_jumpi_neq => OpEntry optimize_jumpi_neq_sbinding optimize_jumpi_neq_sbinding_snd
 end.
 
 Definition all_optimization_steps := 
@@ -580,7 +581,7 @@ Definition all_optimization_steps :=
    OPT_slt_x_x;
    OPT_sgt_x_x
 
-   ;OPT_jumpi_eval
+   ;OPT_jumpi_neq
    ;OPT_mem_solver
    ;OPT_strg_solver
 ].
@@ -653,7 +654,7 @@ Definition all_optimization_steps' :=
    OPT_slt_x_x;
    OPT_sgt_x_x
 
-   ;OPT_jumpi_eval
+   ;OPT_jumpi_neq
    ;OPT_mem_solver
    ;OPT_strg_solver   
 ].
